Working on Nominal still. Almost done.

src/Smty.v
@@ -3,6 +3,8 @@ Require Import Maps.
 Require Import Context.
 Import Context.Context.
 Require Import Coq.Lists.List.
+Require Import Coq.ZArith.ZArith.
+
 
 Module Smty.
 
@@ -26,11 +28,71 @@ Inductive ty : Set :=
     *)
     | TRcd : tyid -> ty -> list (id* ty) -> ty.
 
+Axiom nominal_eq : 
+    forall tid su0 su1 rcd0 rcd1,
+        TRcd tid su0 rcd0 = TRcd tid su1 rcd1. 
+
+(* Scheme Equality for ty. is not working. *)
+Theorem eq_ty_dec (T0 T1:ty) : {T0 = T1} + {T0 <> T1}.
+generalize dependent T1.
+induction T0; intro T1; induction T1;
+
+try 
+(match goal with
+| [|- {?X = ?X} + {_}] => left; auto; fail
+| [|- {_} + {?X <> ?Y}] => right; intro; discriminate
+end).
+    destruct (IHT0_1 T1_1); destruct (IHT0_2 T1_2); subst; try tauto;
+    right; intro K; injection K; subst; auto.
+    destruct (IHT0_1 T1_1); destruct (IHT0_2 T1_2); subst; try tauto;
+    right; intro K; injection K; subst; auto.
+    destruct (eq_id_dec t t0);subst; eauto using nominal_eq.
+    right; intro K; injection K; subst; auto.
+
+Qed.
+
+Definition eq_ty_dec_bool (T0 T1: ty) : bool :=
+    if (eq_ty_dec T0 T1) then true else false.
+
+
+Theorem eq_ty_dec_id:
+    forall t (A: Set) (a b : A),
+        (if eq_ty_dec t t then a else b) = a.
+    intro t. destruct (eq_ty_dec t t); eauto. 
+    destruct (n eq_refl).
+Qed.
+
+Theorem eq_ty_dec_nid:
+    forall t0 t1 (A: Set) (a b : A),
+        t0 <> t1 ->
+        (if eq_ty_dec t0 t1 then a else b) = b.
+
+    intros t0 t1. destruct (eq_ty_dec t0 t1); subst; eauto; try discriminate.
+    intros. destruct (H eq_refl).
+Qed.
+
+Theorem eq_ty_dec_bool_true:
+    forall t ,
+        eq_ty_dec_bool t t = true.
+    unfold eq_ty_dec_bool. intro. eapply eq_ty_dec_id.
+Qed.
+
+Theorem eq_ty_dec_bool_false:
+    forall t0 t1,
+    t0 <> t1 ->
+    eq_ty_dec_bool t0 t1 = false.
+
+    intros t0 t1. eapply eq_ty_dec_nid.
+Qed.
+
+    
+
+
 Inductive tm : Set :=
     | tnone : tm 
     | tif: tm -> tm -> tm -> tm 
     | tvar : id -> tm
-    | tzero : tm
+    | tint : Z -> tm
     | tsuc : tm -> tm 
     | tdec : tm -> tm
     | tngt : tm -> tm -> tm 
@@ -72,14 +134,17 @@ Inductive tm : Set :=
         (*
             TypeA.a :: TypeA -> Int
         *)
-    | tseq : tm -> tm.
+    | tseq : tm -> tm -> tm.
 
+Hint Constructors tm.
 
 
 Inductive inheritable : ty -> Prop :=
 | inh_n : inheritable TNone
 | inh_r : forall c suty l,
             inheritable (TRcd c suty l).
+
+Hint Constructors inheritable.
 
 (* Structual Information will not be checked until 
     type name elimination. *)
@@ -111,5 +176,7 @@ Inductive subty  : ty -> ty -> Prop :=
             subty t0 t1 ->
             subty t1 t2 ->
             subty t0 t2.
+
+Hint Constructors subty.
 
 End Smty.
