src/Context.v
@@ -1,3 +1,4 @@
+Add LoadPath "src".
 Require Import Maps.
 Require Import Coq.Relations.Relation_Definitions.
 Require Import LibTactics.
